Fixed hone representation definitions.

src/ADTRefinement/Refinements/HoneRepresentation.v
@@ -2,7 +2,9 @@ Require Import Fiat.Common
         Fiat.Computation
         Fiat.ADT.ADTSig
         Fiat.ADT.Core
-        Fiat.ADTRefinement.Core Fiat.ADTRefinement.SetoidMorphisms
+        Fiat.ADT.ComputationalADT
+        Fiat.ADTRefinement.Core
+        Fiat.ADTRefinement.SetoidMorphisms
         Fiat.ADTRefinement.GeneralRefinements.
 
 (* A generic refinement and honing tactic for switching the
@@ -21,75 +23,245 @@ Section HoneRepresentation.
      implementation (computation?) for the methods of an ADT by
      using the old methods. *)
 
+  Fixpoint unCurry_Dom
+           (fDom : list Type)
+    : Type :=
+    match fDom with
+    | nil => unit
+    | cons T fDom' => prod T (unCurry_Dom fDom')
+    end.
+
+  Fixpoint unCurry_methodType'
+           (rep : Type)
+           (dom : list Type)
+           {cod : option Type}
+           (f : methodType' rep dom cod)
+           {struct dom}
+    : methodType' rep (cons (unCurry_Dom dom) nil) cod :=
+    match dom return
+          methodType' rep dom cod
+          -> methodType' rep (cons (unCurry_Dom dom) nil) cod
+    with
+    | nil => fun f _ => f
+    | cons T dom' => fun f t => unCurry_methodType' rep dom' (f (fst t)) (snd t)
+    end f.
+
+  Definition unCurried_methodType
+           (arity : nat)
+           (rep : Type)
+           (dom : list Type)
+           (cod : option Type)
+    : Type := Vector.t rep arity -> methodType' rep (cons (unCurry_Dom dom) nil) cod.
+
+  Fixpoint unCurry_methodType
+           (arity : nat)
+           {rep : Type}
+           {dom : list Type}
+           {cod : option Type}
+           (f : methodType arity rep dom cod)
+    : unCurried_methodType arity rep dom cod :=
+    match arity return
+          methodType arity rep dom cod
+          -> unCurried_methodType arity rep dom cod with
+    | 0 => fun meth v => unCurry_methodType' _ _ meth
+    | S n' => fun meth v => unCurry_methodType (arity := n') (meth (Vector.hd v)) (Vector.tl v)
+    end f.
+
+  Fixpoint Curry_methodType'
+           (rep : Type)
+           (dom : list Type)
+           {cod : option Type}
+           (f : methodType' rep (cons (unCurry_Dom dom) nil) cod)
+           {struct dom}
+    : methodType' rep dom cod :=
+    match dom return
+          methodType' rep (cons (unCurry_Dom dom) nil) cod
+          -> methodType' rep dom cod
+    with
+    | nil => fun f => f tt
+    | cons T dom' => fun f t => Curry_methodType' _ (fun t' => f (t, t'))
+    end f.
+
+  Fixpoint Curry_methodType
+           (arity : nat)
+           (rep : Type)
+           (dom : list Type)
+           {cod : option Type}
+           (f : unCurried_methodType arity rep dom cod)
+           {struct arity}
+    : methodType arity rep dom cod :=
+    match arity return
+          unCurried_methodType arity rep dom cod
+          -> methodType arity rep dom cod
+    with
+    | 0 => fun f => Curry_methodType' _ (f (Vector.nil _))
+    | S n' => fun f t => Curry_methodType (fun t' => f (Vector.cons _ t _ t'))
+    end f.
+
+  Lemma refineFunEquiv_unCurry
+        (arity : nat)
+        (rep : Type)
+        (dom : list Type)
+        {cod : option Type}
+    : forall (f : methodType arity rep dom cod),
+      refineMethod eq _ f (Curry_methodType (unCurry_methodType f)).
+  Proof.
+    induction arity; simpl.
+    - induction dom; simpl.
+      + destruct cod; simpl.
+        * intros f [v v'] Comp_v; repeat (computes_to_econstructor; eauto).
+        * intros f v Comp_v; repeat (computes_to_econstructor; eauto).
+      + simpl; intros; eapply IHdom.
+    - simpl; intros; subst; eauto.
+  Qed.
+
+  Lemma refineMethod_Curry_Some
+        {arity : nat}
+        {rep : Type}
+        {dom : list Type}
+        {cod : Type}
+    : forall (f f' : unCurried_methodType arity rep dom (Some cod)),
+      (forall r_ns ds, refine (f r_ns ds) (f' r_ns ds))
+      -> refineMethod_eq rep arity (Curry_methodType f) (Curry_methodType f').
+  Proof.
+    induction arity; simpl; intros.
+    - induction dom; unfold unCurried_methodType in *; intros; simpl in *.
+      + eapply H.
+      + intros; eapply (IHdom (fun r_ns' t' => f r_ns' (d, t')) (fun r_ns' t' => f' r_ns' (d, t') ));
+          eauto.
+    - intros; simpl in *; eauto.
+  Qed.
+  
+  Lemma refineMethod_Curry_None
+        {arity : nat}
+        {rep : Type}
+        {dom : list Type}
+    : forall (f f' : unCurried_methodType arity rep dom None),
+      (forall r_ns ds, refine (f r_ns ds) (f' r_ns ds))
+      -> refineMethod_eq rep arity (Curry_methodType f) (Curry_methodType f').
+  Proof.
+    induction arity; simpl; intros.
+    - induction dom; unfold unCurried_methodType in *; intros; simpl in *.
+      + eapply H.
+      + intros; eapply (IHdom (fun r_ns' t' => f r_ns' (d, t')) (fun r_ns' t' => f' r_ns' (d, t') ));
+          eauto.
+    - intros; simpl in *; eauto.
+  Qed.
+
   Fixpoint absMethod'
            (dom : list Type)
            (cod : option Type)
-    : methodType' oldRep dom cod
-      -> methodType' newRep dom cod :=
+           (oldMeth : methodType' oldRep dom cod)
+           {struct dom}
+    : methodType' newRep (cons (unCurry_Dom dom) nil) cod :=
     match dom return
-          methodType' oldRep dom cod
-          -> methodType' newRep dom cod
+          methodType' oldRep dom cod ->
+          methodType' newRep (cons (unCurry_Dom dom) nil) cod
     with
     | nil =>
       match cod return
             methodType' oldRep [] cod
-            -> methodType' newRep [] cod
+            -> methodType' newRep (cons (unCurry_Dom []) nil) cod
       with
       | Some cod' =>
-        fun oldMethod =>
+        fun oldMeth _ =>
           {nr' | exists or',
-                 oldMethod ↝ or' /\
-                 fst or' ≃ fst nr' /\ snd or' = snd nr'}%comp
+                 oldMeth ↝ or' /\ fst or' ≃ fst nr' /\ snd or' = snd nr'}%comp
       | None =>
-        fun oldMethod =>
+        fun oldMeth _ =>
           {nr' | exists or',
-                 oldMethod ↝ or' /\ or' ≃ nr'}%comp
-      end
+                 oldMeth ↝ or' /\ or' ≃ nr'}%comp
+         end
     | cons d dom' =>
-      fun oldMethod t =>
-        absMethod' dom' cod (oldMethod t)
-    end.
+      fun oldMeth dom'' => absMethod' dom' cod (oldMeth (fst dom'')) (snd dom'')
+    end oldMeth.
 
-  Fixpoint absMethod
-           arity
-           {dom cod}
+  Fixpoint absMethod_Some
+           (arity : nat)
+           (dom : list Type)
+           (cod : Type)
+           (oldMeth : methodType arity oldRep dom (Some cod))
            {struct arity}
-    : methodType arity oldRep dom cod
-      -> methodType arity newRep dom cod.
-  Admitted.
-  (*refine (match arity return
-                  methodType arity oldRep dom cod
-                  -> methodType arity newRep dom cod
-            with
-            | 0 => absMethod' dom cod
-            | S arity' => _
-            end).
-    simpl; intros.
-    admit.
-  Defined. *)
+    : unCurried_methodType arity newRep dom (Some cod) :=
+    match arity return
+          methodType arity oldRep dom (Some cod) ->
+          unCurried_methodType arity newRep dom (Some cod)
+    with
+    | 0 => fun oldMeth _ => absMethod' dom (Some cod) oldMeth
+    | S n' => fun oldMeth reps args v =>
+                forall r_o,
+                  r_o ≃ Vector.hd reps
+                  -> absMethod_Some dom (oldMeth r_o) (Vector.tl reps) args v
+    end oldMeth.
 
-  Lemma refine_absMethod
-        arity
-        (dom : list Type)
-        (cod : option Type)
-        (oldMethod : methodType arity oldRep dom cod)
-  : @refineMethod oldRep newRep AbsR arity _ _
-                   oldMethod
-                   (absMethod arity oldMethod).
-  Proof.
-    induction dom.
-  Admitted.
-  (*- simpl in *; unfold refineMethod, refineMethod',
-                  absMethod, absMethod', refine; intros;
-      destruct cod; intros; computes_to_inv.
-      + destruct (H0 _ H) as [or' [Comp_or [AbsR_or'' eq_or''] ] ].
-        repeat computes_to_econstructor; eauto.
-        destruct v; simpl in *; subst; econstructor.
-      + destruct (H0 _ H) as [or' [Comp_or AbsR_or'' ] ].
-        repeat computes_to_econstructor; eauto.
-    - intro; simpl; intros.
-      eapply (IHdom (fun or => oldMethod or d)); eauto.
-  Qed. *)
+    Fixpoint absMethod_None
+           (arity : nat)
+           (dom : list Type)
+           (oldMeth : methodType arity oldRep dom None)
+           {struct arity}
+    : unCurried_methodType arity newRep dom None :=
+    match arity return
+          methodType arity oldRep dom None ->
+          unCurried_methodType arity newRep dom None
+    with
+    | 0 => fun oldMeth _ => absMethod' dom None oldMeth
+    | S n' => fun oldMeth reps args v =>
+                forall r_o,
+                  r_o ≃ Vector.hd reps
+                  -> absMethod_None dom (oldMeth r_o) (Vector.tl reps) args v
+    end oldMeth.
+
+    Definition absMethod
+               {arity : nat}
+               {dom : list Type}
+               {cod : option Type}
+               (oldMeth : methodType arity oldRep dom cod)
+      : methodType arity newRep dom cod :=
+      Curry_methodType (match cod return
+                              methodType arity oldRep dom cod
+                              -> unCurried_methodType arity newRep dom cod with
+                        | Some cod => absMethod_Some _ (cod := cod)
+                        | None => absMethod_None _
+                        end oldMeth).
+
+    Local Transparent computes_to.
+    Lemma refine_absMethod
+          arity
+          (dom : list Type)
+          (cod : option Type)
+          (oldMethod : methodType arity oldRep dom cod)
+      : @refineMethod oldRep newRep AbsR arity _ _
+                      oldMethod
+                      (absMethod oldMethod).
+    Proof.
+      induction arity.
+      - simpl in *; induction dom; simpl in *.
+        + destruct cod.
+          * unfold absMethod; simpl; intros [r_n' v] Comp_v;
+              computes_to_inv; subst; destruct_ex; intuition subst;
+                simpl in *; subst.
+            computes_to_econstructor; eauto.
+          * unfold absMethod; simpl; intros r_n' Comp_v;
+              computes_to_inv; subst; destruct_ex; intuition subst;
+                simpl in *; subst.
+            computes_to_econstructor; eauto.
+        + intros; unfold absMethod in *; simpl in *.
+          destruct cod;
+            eapply (IHdom (oldMethod d)).
+      - unfold absMethod in *; simpl; intros.
+        pose proof (IHarity (oldMethod r_o)); clear IHarity.
+        destruct cod; simpl in *.
+        + eapply refineMethod_eq_trans; eauto.
+          eapply refineMethod_Curry_Some; simpl; intros.
+          intros v Comp_v.
+          unfold computes_to in Comp_v; apply Comp_v in H; eauto.
+        + eapply refineMethod_eq_trans; eauto.
+          eapply refineMethod_Curry_None; simpl; intros.
+          intros v Comp_v.
+          unfold computes_to in Comp_v; apply Comp_v in H; eauto.
+    Qed.
+
+    Opaque computes_to.
 
   Hint Resolve refine_absMethod.
 
@@ -101,7 +273,7 @@ Section HoneRepresentation.
     refineADT
       (@Build_ADT Sig oldRep oldMeths)
       (@Build_ADT Sig newRep
-                  (fun idx => absMethod _ (oldMeths idx))).
+                  (fun idx => absMethod (oldMeths idx))).
   Proof.
     eapply refineADT_Build_ADT_Rep; eauto.
   Qed.
